src/proofs/no_slashable_blocks/supporting_lemmas/dv_next_preserves_ind_inv/invs_dv_next_1.dfy
@@ -33,21 +33,21 @@ module Invs_DV_Next_1
     import opened Fnc_Invs_1
     import opened Helper_Sets_Lemmas
 
-    lemma lem_inv_all_honest_nodes_is_a_quorum_dv_next(dv: DVState, event: DV_Block_Proposer_Spec.Event, dv': DVState)       
+    lemma lem_inv_all_honest_nodes_is_a_quorum_dv_next(dv: DVState, event: DV_Block_Proposer_Spec.BlockEvent, dv': DVState)       
     requires NextEventPreCond(dv, event)
     requires NextEvent(dv, event, dv')  
     requires inv_all_honest_nodes_is_a_quorum(dv)
     ensures inv_all_honest_nodes_is_a_quorum(dv')
     { }    
 
-    lemma lem_inv_nodes_in_consensus_instances_are_in_dv_dv_next(dv: DVState, event: DV_Block_Proposer_Spec.Event, dv': DVState)       
+    lemma lem_inv_nodes_in_consensus_instances_are_in_dv_dv_next(dv: DVState, event: DV_Block_Proposer_Spec.BlockEvent, dv': DVState)       
     requires NextEventPreCond(dv, event)
     requires NextEvent(dv, event, dv')  
     requires inv_nodes_in_consensus_instances_are_in_dv(dv)
     ensures inv_nodes_in_consensus_instances_are_in_dv(dv')
     { }    
 
-    lemma lem_inv_only_dv_construct_complete_signing_functions_dv_next(dv: DVState, event: DV_Block_Proposer_Spec.Event, dv': DVState)       
+    lemma lem_inv_only_dv_construct_complete_signing_functions_dv_next(dv: DVState, event: DV_Block_Proposer_Spec.BlockEvent, dv': DVState)       
     requires NextEventPreCond(dv, event)
     requires NextEvent(dv, event, dv')  
     requires inv_only_dv_construct_complete_signing_functions(dv)
@@ -56,7 +56,7 @@ module Invs_DV_Next_1
 
     lemma lem_inv_current_proposer_duty_is_a_rcvd_duty_dv_next(
         dv: DVState,
-        event: DV_Block_Proposer_Spec.Event,
+        event: DV_Block_Proposer_Spec.BlockEvent,
         dv': DVState
     )    
     requires NextEventPreCond(dv, event)
@@ -105,7 +105,7 @@ module Invs_DV_Next_1
 
     lemma lem_inv_latest_served_duty_is_a_rcvd_duty_dv_next(
         dv: DVState,
-        event: DV_Block_Proposer_Spec.Event,
+        event: DV_Block_Proposer_Spec.BlockEvent,
         dv': DVState
     )    
     requires NextEventPreCond(dv, event)
@@ -154,7 +154,7 @@ module Invs_DV_Next_1
 
     lemma lem_inv_none_latest_proposer_duty_implies_none_current_proposer_duty_dv_next(
         dv: DVState,
-        event: DV_Block_Proposer_Spec.Event,
+        event: DV_Block_Proposer_Spec.BlockEvent,
         dv': DVState
     )    
     requires NextEventPreCond(dv, event)
@@ -203,7 +203,7 @@ module Invs_DV_Next_1
 
     lemma lem_inv_current_proposer_duty_is_either_none_or_latest_proposer_duty_dv_next(
         dv: DVState,
-        event: DV_Block_Proposer_Spec.Event,
+        event: DV_Block_Proposer_Spec.BlockEvent,
         dv': DVState
     )    
     requires NextEventPreCond(dv, event)
@@ -252,7 +252,7 @@ module Invs_DV_Next_1
 
     lemma lem_inv_available_current_proposer_duty_is_latest_proposer_duty_dv_next(
         dv: DVState,
-        event: DV_Block_Proposer_Spec.Event,
+        event: DV_Block_Proposer_Spec.BlockEvent,
         dv': DVState
     )    
     requires NextEventPreCond(dv, event)
@@ -301,7 +301,7 @@ module Invs_DV_Next_1
 
     lemma lem_inv_seq_of_proposer_duties_is_ordered_dv_next(
         dv: DVState,
-        event: DV_Block_Proposer_Spec.Event,
+        event: DV_Block_Proposer_Spec.BlockEvent,
         dv': DVState
     )    
     requires NextEventPreCond(dv, event)
@@ -314,7 +314,7 @@ module Invs_DV_Next_1
 
     lemma lem_inv_no_duplicated_proposer_duties_dv_next(
         dv: DVState,
-        event: DV_Block_Proposer_Spec.Event,
+        event: DV_Block_Proposer_Spec.BlockEvent,
         dv': DVState
     )    
     requires NextEventPreCond(dv, event)
@@ -325,7 +325,7 @@ module Invs_DV_Next_1
 
     lemma lem_inv_unchanged_dv_seq_of_proposer_duties_dv_next(
         dv: DVState,
-        event: DV_Block_Proposer_Spec.Event,
+        event: DV_Block_Proposer_Spec.BlockEvent,
         dv': DVState
     )    
     requires NextEventPreCond(dv, event)
@@ -337,7 +337,7 @@ module Invs_DV_Next_1
 
     lemma lem_inv_available_latest_proposer_duty_is_from_dv_seq_of_proposer_duties_dv_next(
         dv: DVState,
-        event: DV_Block_Proposer_Spec.Event,
+        event: DV_Block_Proposer_Spec.BlockEvent,
         dv': DVState
     )    
     requires NextEvent.requires(dv, event, dv')  
@@ -451,7 +451,7 @@ module Invs_DV_Next_1
 
     lemma lem_inv_dvc_has_no_active_consensus_instances_if_latest_proposer_duty_is_none_dv_next(
         dv: DVState,
-        event: DV_Block_Proposer_Spec.Event,
+        event: DV_Block_Proposer_Spec.BlockEvent,
         dv': DVState
     )    
     requires NextEventPreCond(dv, event)
@@ -501,9 +501,9 @@ module Invs_DV_Next_1
 
     lemma lem_inv_every_proposer_duty_before_dv_index_next_proposer_duty_to_be_served_was_delivered_f_serve_proposer_duty(
         dv: DVState,
-        event: DV_Block_Proposer_Spec.Event,
+        event: DV_Block_Proposer_Spec.BlockEvent,
         node: BLSPubkey,
-        nodeEvent: Block_Types.Event,
+        nodeEvent: Block_Types.BlockEvent,
         nodeOutputs: DVC_Block_Proposer_Spec_Instr.Outputs,
         dv': DVState
     )  
@@ -576,7 +576,7 @@ module Invs_DV_Next_1
 
     lemma lem_inv_every_proposer_duty_before_dv_index_next_proposer_duty_to_be_served_was_delivered_dv_next(
         dv: DVState,
-        event: DV_Block_Proposer_Spec.Event,
+        event: DV_Block_Proposer_Spec.BlockEvent,
         dv': DVState
     )    
     requires NextEventPreCond(dv, event)
@@ -634,7 +634,7 @@ module Invs_DV_Next_1
 
     lemma lem_inv_dvc_joins_only_consensus_instances_for_which_it_has_received_corresponding_proposer_duties_dv_next(
         dv: DVState,
-        event: DV_Block_Proposer_Spec.Event,
+        event: DV_Block_Proposer_Spec.BlockEvent,
         dv': DVState
     )    
     requires NextEventPreCond(dv, event)
@@ -684,7 +684,7 @@ module Invs_DV_Next_1
     
     lemma lem_inv_the_consensus_instance_indexed_k_is_for_the_rcvd_duty_for_slot_k_dv_next(
         dv: DVState,
-        event: DV_Block_Proposer_Spec.Event,
+        event: DV_Block_Proposer_Spec.BlockEvent,
         dv': DVState
     )    
     requires NextEventPreCond(dv, event)
