src/proofs/no_slashable_blocks/supporting_lemmas/dv_next_preserves_ind_inv/invs_fnc_1 copy.dfy
@@ -36,191 +36,191 @@ module Fnc_Invs_Copy
     import opened DV_Block_Proposer_Spec
     import opened Fnc_Invs_1
 
-    lemma lem_inv_slots_in_slashing_db_are_not_higher_than_the_slot_of_latest_slashing_db_block_body_f_add_block_to_bn(
-        process: DVCState,
-        block: BeaconBlock,
-        process': DVCState 
-    )
-    requires f_add_block_to_bn.requires(process, block)
-    requires process' == f_add_block_to_bn(process, block)    
-    requires inv_slots_in_slashing_db_are_not_higher_than_the_slot_of_latest_slashing_db_block_body(process)
-    ensures inv_slots_in_slashing_db_are_not_higher_than_the_slot_of_latest_slashing_db_block_body(process')
-    { }
+    // lemma lem_inv_slots_in_slashing_db_are_not_higher_than_the_slot_of_latest_slashing_db_block_body_f_add_block_to_bn(
+    //     process: DVCState,
+    //     block: BeaconBlock,
+    //     process': DVCState 
+    // )
+    // requires f_add_block_to_bn.requires(process, block)
+    // requires process' == f_add_block_to_bn(process, block)    
+    // requires inv_slots_in_slashing_db_are_not_higher_than_the_slot_of_latest_slashing_db_block_body(process)
+    // ensures inv_slots_in_slashing_db_are_not_higher_than_the_slot_of_latest_slashing_db_block_body(process')
+    // { }
 
-    lemma lem_inv_slots_in_slashing_db_are_not_higher_than_the_slot_of_latest_slashing_db_block_body_f_terminate_current_proposer_duty(
-        process: DVCState,
-        process': DVCState
-    )
-    requires f_terminate_current_proposer_duty.requires(process)
-    requires process' == f_terminate_current_proposer_duty(process)
-    requires inv_slots_in_slashing_db_are_not_higher_than_the_slot_of_latest_slashing_db_block_body(process)
-    ensures inv_slots_in_slashing_db_are_not_higher_than_the_slot_of_latest_slashing_db_block_body(process')
-    { }
+    // lemma lem_inv_slots_in_slashing_db_are_not_higher_than_the_slot_of_latest_slashing_db_block_body_f_terminate_current_proposer_duty(
+    //     process: DVCState,
+    //     process': DVCState
+    // )
+    // requires f_terminate_current_proposer_duty.requires(process)
+    // requires process' == f_terminate_current_proposer_duty(process)
+    // requires inv_slots_in_slashing_db_are_not_higher_than_the_slot_of_latest_slashing_db_block_body(process)
+    // ensures inv_slots_in_slashing_db_are_not_higher_than_the_slot_of_latest_slashing_db_block_body(process')
+    // { }
 
-    lemma lem_inv_slots_in_slashing_db_are_not_higher_than_the_slot_of_latest_slashing_db_block_body_f_start_consensus_if_can_construct_randao_share(
-        process: DVCState, 
-        process': DVCState)
-    requires f_start_consensus_if_can_construct_randao_share.requires(process)
-    requires process' == f_start_consensus_if_can_construct_randao_share(process).state    
-    requires inv_slots_in_slashing_db_are_not_higher_than_the_slot_of_latest_slashing_db_block_body(process)
-    ensures inv_slots_in_slashing_db_are_not_higher_than_the_slot_of_latest_slashing_db_block_body(process')
-    { }      
+    // lemma lem_inv_slots_in_slashing_db_are_not_higher_than_the_slot_of_latest_slashing_db_block_body_f_start_consensus_if_can_construct_randao_share(
+    //     process: DVCState, 
+    //     process': DVCState)
+    // requires f_start_consensus_if_can_construct_randao_share.requires(process)
+    // requires process' == f_start_consensus_if_can_construct_randao_share(process).state    
+    // requires inv_slots_in_slashing_db_are_not_higher_than_the_slot_of_latest_slashing_db_block_body(process)
+    // ensures inv_slots_in_slashing_db_are_not_higher_than_the_slot_of_latest_slashing_db_block_body(process')
+    // { }      
 
-    lemma lem_inv_slots_in_slashing_db_are_not_higher_than_the_slot_of_latest_slashing_db_block_body_f_listen_for_randao_shares(
-        process: DVCState, 
-        randao_share: RandaoShare,
-        process': DVCState)
-    requires f_listen_for_randao_shares.requires(process, randao_share)
-    requires process' == f_listen_for_randao_shares(process, randao_share).state   
-    requires inv_slots_in_slashing_db_are_not_higher_than_the_slot_of_latest_slashing_db_block_body(process)
-    ensures inv_slots_in_slashing_db_are_not_higher_than_the_slot_of_latest_slashing_db_block_body(process')
-    { 
-        var slot := randao_share.slot;
-        var active_consensus_instances_on_beacon_blocks := process.block_consensus_engine_state.active_consensus_instances_on_beacon_blocks.Keys;
+    // lemma lem_inv_slots_in_slashing_db_are_not_higher_than_the_slot_of_latest_slashing_db_block_body_f_listen_for_randao_shares(
+    //     process: DVCState, 
+    //     randao_share: RandaoShare,
+    //     process': DVCState)
+    // requires f_listen_for_randao_shares.requires(process, randao_share)
+    // requires process' == f_listen_for_randao_shares(process, randao_share).state   
+    // requires inv_slots_in_slashing_db_are_not_higher_than_the_slot_of_latest_slashing_db_block_body(process)
+    // ensures inv_slots_in_slashing_db_are_not_higher_than_the_slot_of_latest_slashing_db_block_body(process')
+    // { 
+    //     var slot := randao_share.slot;
+    //     var active_consensus_instances_on_beacon_blocks := process.block_consensus_engine_state.active_consensus_instances_on_beacon_blocks.Keys;
 
-        if is_slot_for_current_or_future_instances(process, slot) 
-        {
-            var process_with_new_randao_share := 
-                process.(
-                    rcvd_randao_shares := process.rcvd_randao_shares[slot := getOrDefault(process.rcvd_randao_shares, slot, {}) + 
-                                                                                    {randao_share} ]
-                );   
-            lem_inv_slots_in_slashing_db_are_not_higher_than_the_slot_of_latest_slashing_db_block_body_f_start_consensus_if_can_construct_randao_share(
-                process_with_new_randao_share,
-                process'
-            );
-        }
-        else
-        { }
-    }      
+    //     if is_slot_for_current_or_future_instances(process, slot) 
+    //     {
+    //         var process_with_new_randao_share := 
+    //             process.(
+    //                 rcvd_randao_shares := process.rcvd_randao_shares[slot := getOrDefault(process.rcvd_randao_shares, slot, {}) + 
+    //                                                                                 {randao_share} ]
+    //             );   
+    //         lem_inv_slots_in_slashing_db_are_not_higher_than_the_slot_of_latest_slashing_db_block_body_f_start_consensus_if_can_construct_randao_share(
+    //             process_with_new_randao_share,
+    //             process'
+    //         );
+    //     }
+    //     else
+    //     { }
+    // }      
 
-    lemma lem_inv_slots_in_slashing_db_are_not_higher_than_the_slot_of_latest_slashing_db_block_body_f_check_for_next_duty(
-        process: DVCState,
-        proposer_duty: ProposerDuty,
-        process': DVCState
-    )
-    requires f_check_for_next_duty.requires(process, proposer_duty)
-    requires process' == f_check_for_next_duty(process, proposer_duty).state
-    requires inv_slots_in_slashing_db_are_not_higher_than_the_slot_of_latest_slashing_db_block_body(process)
-    ensures inv_slots_in_slashing_db_are_not_higher_than_the_slot_of_latest_slashing_db_block_body(process')
-    { }
+    // lemma lem_inv_slots_in_slashing_db_are_not_higher_than_the_slot_of_latest_slashing_db_block_body_f_check_for_next_duty(
+    //     process: DVCState,
+    //     proposer_duty: ProposerDuty,
+    //     process': DVCState
+    // )
+    // requires f_check_for_next_duty.requires(process, proposer_duty)
+    // requires process' == f_check_for_next_duty(process, proposer_duty).state
+    // requires inv_slots_in_slashing_db_are_not_higher_than_the_slot_of_latest_slashing_db_block_body(process)
+    // ensures inv_slots_in_slashing_db_are_not_higher_than_the_slot_of_latest_slashing_db_block_body(process')
+    // { }
 
-    lemma lem_inv_slots_in_slashing_db_are_not_higher_than_the_slot_of_latest_slashing_db_block_body_f_broadcast_randao_share(
-        process: DVCState,
-        proposer_duty: ProposerDuty, 
-        process': DVCState
-    )
-    requires f_broadcast_randao_share.requires(process, proposer_duty)
-    requires process' == f_broadcast_randao_share(process, proposer_duty).state
-    requires inv_slots_in_slashing_db_are_not_higher_than_the_slot_of_latest_slashing_db_block_body(process)
-    ensures inv_slots_in_slashing_db_are_not_higher_than_the_slot_of_latest_slashing_db_block_body(process')
-    { 
-        var slot := proposer_duty.slot;
-        var fork_version := bn_get_fork_version(slot);    
-        var epoch := compute_epoch_at_slot(slot);
-        var randao_reveal_signing_root := compute_randao_reveal_signing_root(slot);
-        var randao_reveal_signature_share := rs_sign_randao_reveal(epoch, fork_version, randao_reveal_signing_root, process.rs);
-        var randao_share := 
-            RandaoShare(
-                proposer_duty := proposer_duty,
-                slot := slot,
-                signing_root := randao_reveal_signing_root,
-                signature := randao_reveal_signature_share
-            );
-        var process_after_adding_randao_share :=
-            process.(
-                randao_shares_to_broadcast := process.randao_shares_to_broadcast[proposer_duty.slot := randao_share]
-            );
+    // lemma lem_inv_slots_in_slashing_db_are_not_higher_than_the_slot_of_latest_slashing_db_block_body_f_broadcast_randao_share(
+    //     process: DVCState,
+    //     proposer_duty: ProposerDuty, 
+    //     process': DVCState
+    // )
+    // requires f_broadcast_randao_share.requires(process, proposer_duty)
+    // requires process' == f_broadcast_randao_share(process, proposer_duty).state
+    // requires inv_slots_in_slashing_db_are_not_higher_than_the_slot_of_latest_slashing_db_block_body(process)
+    // ensures inv_slots_in_slashing_db_are_not_higher_than_the_slot_of_latest_slashing_db_block_body(process')
+    // { 
+    //     var slot := proposer_duty.slot;
+    //     var fork_version := bn_get_fork_version(slot);    
+    //     var epoch := compute_epoch_at_slot(slot);
+    //     var randao_reveal_signing_root := compute_randao_reveal_signing_root(slot);
+    //     var randao_reveal_signature_share := rs_sign_randao_reveal(epoch, fork_version, randao_reveal_signing_root, process.rs);
+    //     var randao_share := 
+    //         RandaoShare(
+    //             proposer_duty := proposer_duty,
+    //             slot := slot,
+    //             signing_root := randao_reveal_signing_root,
+    //             signature := randao_reveal_signature_share
+    //         );
+    //     var process_after_adding_randao_share :=
+    //         process.(
+    //             randao_shares_to_broadcast := process.randao_shares_to_broadcast[proposer_duty.slot := randao_share]
+    //         );
 
-        lem_inv_slots_in_slashing_db_are_not_higher_than_the_slot_of_latest_slashing_db_block_body_f_check_for_next_duty(
-            process_after_adding_randao_share,
-            proposer_duty,
-            process'
-        );
-    }
+    //     lem_inv_slots_in_slashing_db_are_not_higher_than_the_slot_of_latest_slashing_db_block_body_f_check_for_next_duty(
+    //         process_after_adding_randao_share,
+    //         proposer_duty,
+    //         process'
+    //     );
+    // }
 
-    lemma lem_inv_slots_in_slashing_db_are_not_higher_than_the_slot_of_latest_slashing_db_block_body_f_serve_proposer_duty(
-        process: DVCState,
-        proposer_duty: ProposerDuty,
-        process': DVCState
-    )  
-    requires f_serve_proposer_duty.requires(process, proposer_duty)
-    requires process' == f_serve_proposer_duty(process, proposer_duty).state
-    requires inv_slots_in_slashing_db_are_not_higher_than_the_slot_of_latest_slashing_db_block_body(process)
-    ensures inv_slots_in_slashing_db_are_not_higher_than_the_slot_of_latest_slashing_db_block_body(process')
-    {
-        var process_after_stopping_current_duty := f_terminate_current_proposer_duty(process);
+    // lemma lem_inv_slots_in_slashing_db_are_not_higher_than_the_slot_of_latest_slashing_db_block_body_f_serve_proposer_duty(
+    //     process: DVCState,
+    //     proposer_duty: ProposerDuty,
+    //     process': DVCState
+    // )  
+    // requires f_serve_proposer_duty.requires(process, proposer_duty)
+    // requires process' == f_serve_proposer_duty(process, proposer_duty).state
+    // requires inv_slots_in_slashing_db_are_not_higher_than_the_slot_of_latest_slashing_db_block_body(process)
+    // ensures inv_slots_in_slashing_db_are_not_higher_than_the_slot_of_latest_slashing_db_block_body(process')
+    // {
+    //     var process_after_stopping_current_duty := f_terminate_current_proposer_duty(process);
         
-        lem_inv_slots_in_slashing_db_are_not_higher_than_the_slot_of_latest_slashing_db_block_body_f_terminate_current_proposer_duty(
-            process,
-            process_after_stopping_current_duty
-        );
+    //     lem_inv_slots_in_slashing_db_are_not_higher_than_the_slot_of_latest_slashing_db_block_body_f_terminate_current_proposer_duty(
+    //         process,
+    //         process_after_stopping_current_duty
+    //     );
 
-        var process_after_receiving_duty := 
-            f_receive_new_duty(process_after_stopping_current_duty, proposer_duty);
+    //     var process_after_receiving_duty := 
+    //         f_receive_new_duty(process_after_stopping_current_duty, proposer_duty);
        
-        lem_inv_slots_in_slashing_db_are_not_higher_than_the_slot_of_latest_slashing_db_block_body_f_broadcast_randao_share(
-            process_after_receiving_duty,
-            proposer_duty,
-            process'
-        );
-    } 
+    //     lem_inv_slots_in_slashing_db_are_not_higher_than_the_slot_of_latest_slashing_db_block_body_f_broadcast_randao_share(
+    //         process_after_receiving_duty,
+    //         proposer_duty,
+    //         process'
+    //     );
+    // } 
 
-    lemma lem_inv_slots_in_slashing_db_are_not_higher_than_the_slot_of_latest_slashing_db_block_body_f_block_consensus_decided(
-        process: DVCState,
-        id: Slot,
-        block: BeaconBlock, 
-        process': DVCState
-    )
-    requires f_block_consensus_decided.requires(process, id, block)
-    requires process' == f_block_consensus_decided(process, id, block).state 
-    requires inv_slots_in_slashing_db_are_not_higher_than_the_slot_of_latest_slashing_db_block_body(process)
-    ensures inv_slots_in_slashing_db_are_not_higher_than_the_slot_of_latest_slashing_db_block_body(process')
-    { }  
+    // lemma lem_inv_slots_in_slashing_db_are_not_higher_than_the_slot_of_latest_slashing_db_block_body_f_block_consensus_decided(
+    //     process: DVCState,
+    //     id: Slot,
+    //     block: BeaconBlock, 
+    //     process': DVCState
+    // )
+    // requires f_block_consensus_decided.requires(process, id, block)
+    // requires process' == f_block_consensus_decided(process, id, block).state 
+    // requires inv_slots_in_slashing_db_are_not_higher_than_the_slot_of_latest_slashing_db_block_body(process)
+    // ensures inv_slots_in_slashing_db_are_not_higher_than_the_slot_of_latest_slashing_db_block_body(process')
+    // { }  
 
-    lemma lem_inv_slots_in_slashing_db_are_not_higher_than_the_slot_of_latest_slashing_db_block_body_f_listen_for_block_signature_shares(
-        process: DVCState,
-        block_share: SignedBeaconBlock,
-        process': DVCState
-    )
-    requires f_listen_for_block_signature_shares.requires(process, block_share)
-    requires process' == f_listen_for_block_signature_shares(process, block_share).state
-    requires inv_slots_in_slashing_db_are_not_higher_than_the_slot_of_latest_slashing_db_block_body(process)
-    ensures inv_slots_in_slashing_db_are_not_higher_than_the_slot_of_latest_slashing_db_block_body(process')
-    { }
+    // lemma lem_inv_slots_in_slashing_db_are_not_higher_than_the_slot_of_latest_slashing_db_block_body_f_listen_for_block_signature_shares(
+    //     process: DVCState,
+    //     block_share: SignedBeaconBlock,
+    //     process': DVCState
+    // )
+    // requires f_listen_for_block_signature_shares.requires(process, block_share)
+    // requires process' == f_listen_for_block_signature_shares(process, block_share).state
+    // requires inv_slots_in_slashing_db_are_not_higher_than_the_slot_of_latest_slashing_db_block_body(process)
+    // ensures inv_slots_in_slashing_db_are_not_higher_than_the_slot_of_latest_slashing_db_block_body(process')
+    // { }
 
-    lemma lem_inv_slots_in_slashing_db_are_not_higher_than_the_slot_of_latest_slashing_db_block_body_f_listen_for_new_imported_blocks(
-        process: DVCState,
-        block: BeaconBlock,
-        process': DVCState
-    )
-    requires f_listen_for_new_imported_blocks.requires(process, block)
-    requires process' == f_listen_for_new_imported_blocks(process, block).state
-    requires inv_slots_in_slashing_db_are_not_higher_than_the_slot_of_latest_slashing_db_block_body(process)
-    ensures inv_slots_in_slashing_db_are_not_higher_than_the_slot_of_latest_slashing_db_block_body(process')
-    { }  
+    // lemma lem_inv_slots_in_slashing_db_are_not_higher_than_the_slot_of_latest_slashing_db_block_body_f_listen_for_new_imported_blocks(
+    //     process: DVCState,
+    //     block: BeaconBlock,
+    //     process': DVCState
+    // )
+    // requires f_listen_for_new_imported_blocks.requires(process, block)
+    // requires process' == f_listen_for_new_imported_blocks(process, block).state
+    // requires inv_slots_in_slashing_db_are_not_higher_than_the_slot_of_latest_slashing_db_block_body(process)
+    // ensures inv_slots_in_slashing_db_are_not_higher_than_the_slot_of_latest_slashing_db_block_body(process')
+    // { }  
 
-    lemma lem_inv_slots_in_slashing_db_are_not_higher_than_the_slot_of_latest_slashing_db_block_body_f_resend_randao_share(
-        process: DVCState, 
-        process': DVCState)
-    requires f_resend_randao_share.requires(process)
-    requires process' == f_resend_randao_share(process).state    
-    requires inv_slots_in_slashing_db_are_not_higher_than_the_slot_of_latest_slashing_db_block_body(process)
-    ensures inv_slots_in_slashing_db_are_not_higher_than_the_slot_of_latest_slashing_db_block_body(process')
-    { }  
+    // lemma lem_inv_slots_in_slashing_db_are_not_higher_than_the_slot_of_latest_slashing_db_block_body_f_resend_randao_share(
+    //     process: DVCState, 
+    //     process': DVCState)
+    // requires f_resend_randao_share.requires(process)
+    // requires process' == f_resend_randao_share(process).state    
+    // requires inv_slots_in_slashing_db_are_not_higher_than_the_slot_of_latest_slashing_db_block_body(process)
+    // ensures inv_slots_in_slashing_db_are_not_higher_than_the_slot_of_latest_slashing_db_block_body(process')
+    // { }  
 
-    lemma lem_inv_slots_in_slashing_db_are_not_higher_than_the_slot_of_latest_slashing_db_block_body_f_resend_block_share(
-        process: DVCState, 
-        process': DVCState)
-    requires f_resend_block_share.requires(process)
-    requires process' == f_resend_block_share(process).state    
-    requires inv_slots_in_slashing_db_are_not_higher_than_the_slot_of_latest_slashing_db_block_body(process)
-    ensures inv_slots_in_slashing_db_are_not_higher_than_the_slot_of_latest_slashing_db_block_body(process')
-    { }  
+    // lemma lem_inv_slots_in_slashing_db_are_not_higher_than_the_slot_of_latest_slashing_db_block_body_f_resend_block_share(
+    //     process: DVCState, 
+    //     process': DVCState)
+    // requires f_resend_block_share.requires(process)
+    // requires process' == f_resend_block_share(process).state    
+    // requires inv_slots_in_slashing_db_are_not_higher_than_the_slot_of_latest_slashing_db_block_body(process)
+    // ensures inv_slots_in_slashing_db_are_not_higher_than_the_slot_of_latest_slashing_db_block_body(process')
+    // { }  
 
     // lemma lem_inv_slots_in_slashing_db_are_not_higher_than_the_slot_of_latest_slashing_db_block_dv_next(
     //     dv: DVState,
-    //     event: DV_Block_Proposer_Spec.Event,
+    //     event: DV_Block_Proposer_Spec.BlockEvent,
     //     dv': DVState
     // )    
     // requires NextEventPreCond(dv, event)
